Boolean relations on iformulas

yalla/iformulas.v
@@ -6,7 +6,10 @@
 
 Require Import RelationClasses.
 Require Import List.
+Require Import Bool.
 Require Import Omega.
+
+Require Import Bool_more.
 
 Require yalla_ax.
 
@@ -75,8 +78,7 @@ Inductive isubform : iformula -> iformula -> Prop :=
 | isub_lpam_r : forall A B C, isubform A B -> isubform A (ilpam C B)
 | isub_lmap_l : forall A B C, isubform A B -> isubform A (ilmap B C)
 | isub_lmap_r : forall A B C, isubform A B -> isubform A (ilmap C B)
-| isub_neg_l  : forall A B, isubform A B -> isubform A (ineg B)
-| isub_neg_r  : forall A B, isubform A B -> isubform A (ineg B)
+| isub_neg    : forall A B, isubform A B -> isubform A (ineg B)
 | isub_neg_N  : forall A, isubform N (ineg A)
 | isub_plus_l : forall A B C, isubform A B -> isubform A (iplus B C)
 | isub_plus_r : forall A B C, isubform A B -> isubform A (iplus C B)
@@ -165,4 +167,318 @@ intros b l l1 l2 H1 HP ; revert H1 ; induction l ; intro H1.
   + apply IHl...
 Qed.
 *)
+
+
+(** ** Equality in [bool] *)
+
+Fixpoint eqb_iform A B :=
+match A, B with
+| ivar X, ivar Y => yalla_ax.iateq X Y
+| ione, ione => true
+| itens A1 A2, itens B1 B2 => (eqb_iform A1 B1) && (eqb_iform A2 B2)
+| ilpam A1 A2, ilpam B1 B2 => (eqb_iform A1 B1) && (eqb_iform A2 B2)
+| ilmap A1 A2, ilmap B1 B2 => (eqb_iform A1 B1) && (eqb_iform A2 B2)
+| ineg A1, ineg B1 => eqb_iform A1 B1
+| itop, itop => true
+| izero, izero => true
+| iwith A1 A2, iwith B1 B2 => (eqb_iform A1 B1) && (eqb_iform A2 B2)
+| iplus A1 A2, iplus B1 B2 => (eqb_iform A1 B1) && (eqb_iform A2 B2)
+| ioc A1, ioc B1 => eqb_iform A1 B1
+| _, _ => false
+end.
+
+Lemma eqb_eq_iform : forall A B, eqb_iform A B = true <-> A = B.
+Proof with reflexivity.
+induction A ; destruct B ; (split ; [ intros Heqb | intros Heq ]) ;
+  try inversion Heqb ; try inversion Heq ; try reflexivity.
+- apply yalla_ax.iateq_eq in H0 ; subst...
+- subst ; simpl.
+  apply yalla_ax.iateq_eq...
+- apply andb_true_iff in H0.
+  destruct H0 as [H1 H2].
+  apply IHA1 in H1 ; apply IHA2 in H2 ; subst...
+- subst ; simpl ; apply andb_true_iff.
+  split ; [ apply IHA1 | apply IHA2 ]...
+- apply andb_true_iff in H0.
+  destruct H0 as [H1 H2].
+  apply IHA1 in H1 ; apply IHA2 in H2 ; subst...
+- subst ; simpl ; apply andb_true_iff.
+  split ; [ apply IHA1 | apply IHA2 ]...
+- apply andb_true_iff in H0.
+  destruct H0 as [H1 H2].
+  apply IHA1 in H1 ; apply IHA2 in H2 ; subst...
+- subst ; simpl ; apply andb_true_iff.
+  split ; [ apply IHA1 | apply IHA2 ]...
+- apply IHA in H0 ; subst...
+- subst ; simpl ; apply IHA...
+- apply andb_true_iff in H0.
+  destruct H0 as [H1 H2].
+  apply IHA1 in H1 ; apply IHA2 in H2 ; subst...
+- subst ; simpl ; apply andb_true_iff.
+  split ; [ apply IHA1 | apply IHA2 ]...
+- apply andb_true_iff in H0.
+  destruct H0 as [H1 H2].
+  apply IHA1 in H1 ; apply IHA2 in H2 ; subst...
+- subst ; simpl ; apply andb_true_iff.
+  split ; [ apply IHA1 | apply IHA2 ]...
+- apply IHA in H0 ; subst...
+- subst ; simpl ; apply IHA...
+Qed.
+
+Fixpoint eqb_iformlist l1 l2 :=
+match l1, l2 with
+| nil, nil => true
+| cons A t1, cons B t2 => (eqb_iform A B) && (eqb_iformlist t1 t2)
+| _, _ => false
+end.
+
+Lemma eqb_eq_iformlist : forall l1 l2, eqb_iformlist l1 l2 = true <-> l1 = l2.
+Proof with reflexivity.
+induction l1 ; destruct l2 ; (split ; [ intros Heqb | intros Heq ]) ;
+  try inversion Heqb ; try inversion Heq ; try reflexivity.
+- apply andb_true_iff in H0.
+  destruct H0 as [H1 H2].
+  apply eqb_eq_iform in H1 ; apply IHl1 in H2 ; subst...
+- subst ; simpl ; apply andb_true_iff.
+  split ; [ apply eqb_eq_iform | apply IHl1 ]...
+Qed.
+
+(** * In with [bool] output for formula list *)
+Fixpoint inb_iform A l :=
+match l with
+| nil => false
+| cons hd tl => eqb_iform A hd || inb_iform A tl
+end.
+
+Lemma inb_in_iform : forall A l, inb_iform A l = true <-> In A l.
+Proof with assumption.
+induction l ; (split ; [ intros Heqb | intros Heq ]).
+- inversion Heqb.
+- inversion Heq.
+- inversion Heqb ; subst.
+  apply orb_true_iff in H0.
+  destruct H0.
+  + constructor.
+    symmetry ; apply eqb_eq_iform...
+  + apply in_cons.
+    apply IHl...
+- inversion Heq ; subst.
+  + simpl ; apply orb_true_iff ; left.
+    apply eqb_eq_iform.
+    reflexivity.
+  + simpl ; apply orb_true_iff ; right.
+    apply IHl...
+Qed.
+
+
+(** ** Sub-formulas in [bool] *)
+
+(** First argument is a sub-formula of the second: *)
+Fixpoint isubformb A B :=
+eqb_iform A B ||
+match B with
+| itens B1 B2 => isubformb A B1 || isubformb A B2
+| ilpam B1 B2 => isubformb A B1 || isubformb A B2
+| ilmap B1 B2 => isubformb A B1 || isubformb A B2
+| ineg B1 => isubformb A B1 || eqb_iform A N
+| iwith B1 B2 => isubformb A B1 || isubformb A B2
+| iplus B1 B2 => isubformb A B1 || isubformb A B2
+| ioc B1 => isubformb A B1
+| _ => false
+end.
+
+Lemma isubb_isub : forall A B, is_true (isubformb A B) <-> isubform A B.
+Proof with try assumption ; try reflexivity.
+intros A B ; split ; intros H ; induction B ; try (now (inversion H ; constructor)).
+- destruct A ; simpl in H ; try (now inversion H).
+  rewrite orb_false_r in H.
+  apply yalla_ax.iateq_eq in H ; subst ; constructor.
+- destruct A ; simpl in H ; try (now inversion H).
+- simpl in H.
+  apply orb_true_elim in H ; destruct H as [ H | H ] ;
+    [ | apply orb_true_elim in H ; destruct H as [ H | H ] ].
+  + apply eqb_eq_iform in H ; subst ; constructor.
+  + apply isub_tens_l.
+    apply IHB1...
+  + apply isub_tens_r.
+    apply IHB2...
+- simpl in H.
+  apply orb_true_elim in H ; destruct H as [ H | H ] ;
+    [ | apply orb_true_elim in H ; destruct H as [ H | H ] ].
+  + apply eqb_eq_iform in H ; subst ; constructor.
+  + apply isub_lpam_l.
+    apply IHB1...
+  + apply isub_lpam_r.
+    apply IHB2...
+- simpl in H.
+  apply orb_true_elim in H ; destruct H as [ H | H ] ;
+    [ | apply orb_true_elim in H ; destruct H as [ H | H ] ].
+  + apply eqb_eq_iform in H ; subst ; constructor.
+  + apply isub_lmap_l.
+    apply IHB1...
+  + apply isub_lmap_r.
+    apply IHB2...
+- simpl in H.
+  apply orb_true_elim in H ; destruct H as [ H | H ] ;
+    [ | apply orb_true_elim in H ; destruct H as [ H | H ] ].
+  + apply eqb_eq_iform in H ; subst ; constructor.
+  + apply isub_neg.
+    apply IHB...
+  + apply eqb_eq_iform in H ; subst.
+    apply isub_neg_N.
+- destruct A ; simpl in H ; try (now inversion H).
+- simpl in H.
+  apply orb_true_elim in H ; destruct H as [ H | H ] ;
+    [ | apply orb_true_elim in H ; destruct H as [ H | H ] ].
+  + apply eqb_eq_iform in H ; subst ; constructor.
+  + apply isub_with_l.
+    apply IHB1...
+  + apply isub_with_r.
+    apply IHB2...
+- destruct A ; simpl in H ; try (now inversion H).
+- simpl in H.
+  apply orb_true_elim in H ; destruct H as [ H | H ] ;
+    [ | apply orb_true_elim in H ; destruct H as [ H | H ] ].
+  + apply eqb_eq_iform in H ; subst ; constructor.
+  + apply isub_plus_l.
+    apply IHB1...
+  + apply isub_plus_r.
+    apply IHB2...
+- simpl in H.
+  apply orb_true_elim in H ; destruct H as [ H | H ].
+  + apply eqb_eq_iform in H ; subst ; constructor.
+  + apply isub_oc.
+    apply IHB...
+- inversion H ; subst.
+  simpl ; unfold yalla_ax.iateq ;
+    destruct i ; simpl ; [ | reflexivity ].
+  rewrite <- beq_nat_refl.
+  constructor.
+- inversion H ; subst.
+  + unfold isubformb.
+    replace (eqb_iform (itens B1 B2) (itens B1 B2)) with true...
+    symmetry ; apply eqb_eq_iform...
+  + apply IHB1 in H2.
+    simpl ; rewrite H2 ; simpl.
+    rewrite orb_true_r...
+  + apply IHB2 in H2.
+    simpl ; rewrite H2 ; simpl.
+    rewrite 2 orb_true_r...
+- inversion H ; subst.
+  + unfold isubformb.
+    replace (eqb_iform (ilpam B1 B2) (ilpam B1 B2)) with true...
+    symmetry ; apply eqb_eq_iform...
+  + apply IHB1 in H2.
+    simpl ; rewrite H2 ; simpl.
+    rewrite orb_true_r...
+  + apply IHB2 in H2.
+    simpl ; rewrite H2 ; simpl.
+    rewrite 2 orb_true_r...
+- inversion H ; subst.
+  + unfold isubformb.
+    replace (eqb_iform (ilmap B1 B2) (ilmap B1 B2)) with true...
+    symmetry ; apply eqb_eq_iform...
+  + apply IHB1 in H2.
+    simpl ; rewrite H2 ; simpl.
+    rewrite orb_true_r...
+  + apply IHB2 in H2.
+    simpl ; rewrite H2 ; simpl.
+    rewrite 2 orb_true_r...
+- inversion H ; subst.
+  + unfold isubformb.
+    replace (eqb_iform (ineg B) (ineg B)) with true...
+    symmetry ; apply eqb_eq_iform...
+  + apply IHB in H2.
+    simpl ; rewrite H2 ; simpl.
+    rewrite orb_true_r...
+  + simpl.
+    rewrite orb_true_r...
+- inversion H ; subst.
+  + unfold isubformb.
+    replace (eqb_iform (iwith B1 B2) (iwith B1 B2)) with true...
+    symmetry ; apply eqb_eq_iform...
+  + apply IHB1 in H2.
+    simpl ; rewrite H2 ; simpl.
+    rewrite orb_true_r...
+  + apply IHB2 in H2.
+    simpl ; rewrite H2 ; simpl.
+    rewrite 2 orb_true_r...
+- inversion H ; subst.
+  + unfold isubformb.
+    replace (eqb_iform (iplus B1 B2) (iplus B1 B2)) with true...
+    symmetry ; apply eqb_eq_iform...
+  + apply IHB1 in H2.
+    simpl ; rewrite H2 ; simpl.
+    rewrite orb_true_r...
+  + apply IHB2 in H2.
+    simpl ; rewrite H2 ; simpl.
+    rewrite 2 orb_true_r...
+- inversion H ; subst.
+  + unfold isubformb.
+    replace (eqb_iform (ioc B) (ioc B)) with true...
+    symmetry ; apply eqb_eq_iform...
+  + apply IHB in H2.
+    simpl ; rewrite H2 ; simpl.
+    rewrite orb_true_r...
+Qed.
+
+Lemma isubb_trans : forall A B C,
+  is_true (isubformb A B) -> is_true (isubformb B C) -> is_true (isubformb A C).
+Proof.
+intros A B C Hl Hr.
+apply isubb_isub in Hl.
+apply isubb_isub in Hr.
+apply isubb_isub.
+etransitivity ; eassumption.
+Qed.
+
+(** Each element of the first list is a sub-formula of some element of the second. *)
+Definition isubformb_list l1 l2 := Forallb (fun A => Existsb (isubformb A) l2) l1.
+
+Lemma isubb_isub_list : forall l1 l2, is_true (isubformb_list l1 l2) <-> isubform_list l1 l2.
+Proof with try assumption.
+intros l1 l2 ; split ; intros H ; induction l1 ; try (now (inversion H ; constructor)).
+- unfold isubformb_list in H.
+  apply Forallb_Forall in H.
+  inversion H ; subst.
+  apply Existsb_Exists in H2.
+  constructor.
+  + clear - H2 ; induction l2 ; inversion H2 ; subst.
+    * constructor.
+      apply isubb_isub...
+    * apply Exists_cons_tl.
+      apply IHl2...
+  + apply IHl1.
+    apply Forallb_Forall...
+- inversion H ; subst.
+  unfold isubformb_list ; simpl.
+  apply andb_true_iff ; split.
+  + apply Existsb_Exists.
+    clear - H2 ; induction l2 ; inversion H2 ; subst.
+    * constructor.
+      apply isubb_isub...
+    * apply Exists_cons_tl.
+      apply IHl2...
+  + apply IHl1...
+Qed.
+
+Lemma isubb_id_list : forall l l0, is_true (isubformb_list l (l0 ++ l)).
+Proof.
+intros l l0.
+apply isubb_isub_list.
+apply isub_id_list.
+Qed.
+
+Lemma isubb_trans_list : forall l1 l2 l3,
+  is_true (isubformb_list l1 l2) -> is_true (isubformb_list l2 l3) -> is_true (isubformb_list l1 l3).
+Proof.
+intros l1 l2 l3 Hl Hr.
+apply isubb_isub_list in Hl.
+apply isubb_isub_list in Hr.
+apply isubb_isub_list.
+etransitivity ; eassumption.
+Qed.
+
+
+
 
